AnnotatedBool.v
@@ -19,23 +19,31 @@ Proof.
 Qed.
 
 Lemma annotated_reducible_ite:
-  forall tvars gamma b t1 t2 T x,
-    ~(x ∈ fv_context gamma) ->
-    ~(x ∈ fv b) ->
-    ~(x ∈ fv t1) ->
-    ~(x ∈ fv t2) ->
-    ~(x ∈ fv T) ->
-    ~(x ∈ tvars) ->
+  forall tvars gamma b t1 t2 T x1 x2,
+
+    ~(x1 ∈ fv_context gamma) ->
+    ~(x1 ∈ fv b) ->
+    ~(x1 ∈ fv t1) ->
+    ~(x1 ∈ fv T) ->
+    ~(x1 ∈ tvars) ->
+
+    ~(x2 ∈ fv_context gamma) ->
+    ~(x2 ∈ fv b) ->
+    ~(x2 ∈ fv t2) ->
+    ~(x2 ∈ fv T) ->
+    ~(x2 ∈ tvars) ->
+
     wf t1 0 ->
     wf t2 0 ->
     subset (fv t1) (support gamma) ->
     subset (fv t2) (support gamma) ->
     [[ tvars; gamma ⊨ b : T_bool ]] ->
-    [[ tvars; (x, T_equiv b ttrue)  :: gamma ⊨ t1 : T ]] ->
-    [[ tvars; (x, T_equiv b tfalse) :: gamma ⊨ t2 : T ]] ->
+    [[ tvars; (x1, T_equiv b ttrue)  :: gamma ⊨ t1 : T ]] ->
+    [[ tvars; (x2, T_equiv b tfalse) :: gamma ⊨ t2 : T ]] ->
     [[ tvars; gamma ⊨ ite b t1 t2 : T ]].
 Proof.
-  unfold annotated_reducible;
-    repeat step || apply open_reducible_ite with x;
+  unfold annotated_reducible.
+  repeat step.
+    repeat step || apply open_reducible_ite with (x1 := x1) (x2 := x2);
     side_conditions.
 Qed.
