AnnotatedIte.v
@@ -3,14 +3,19 @@ Require Export SystemFR.AnnotatedTactics.
 Require Export SystemFR.ErasedIte.
 
 Lemma annotated_reducible_T_ite:
-  forall tvars gamma b t1 t2 T1 T2 x,
-    ~(x ∈ fv_context gamma) ->
-    ~(x ∈ fv b) ->
-    ~(x ∈ fv t1) ->
-    ~(x ∈ fv t2) ->
-    ~(x ∈ fv T1) ->
-    ~(x ∈ fv T2) ->
-    ~(x ∈ tvars) ->
+  forall tvars gamma b t1 t2 T1 T2 x1 x2,
+    ~(x1 ∈ fv_context gamma) ->
+    ~(x1 ∈ fv b) ->
+    ~(x1 ∈ fv t1) ->
+    ~(x1 ∈ fv T1) ->
+    ~(x1 ∈ tvars) ->
+
+    ~(x2 ∈ fv_context gamma) ->
+    ~(x2 ∈ fv b) ->
+    ~(x2 ∈ fv t2) ->
+    ~(x2 ∈ fv T2) ->
+    ~(x2 ∈ tvars) ->
+
     wf t1 0 ->
     wf t2 0 ->
     wf T1 0 ->
@@ -21,14 +26,14 @@ Lemma annotated_reducible_T_ite:
     subset (fv T1) (support gamma) ->
     subset (fv T2) (support gamma) ->
     [[ tvars; gamma ⊨ b : T_bool ]] ->
-    [[ tvars; (x, T_equiv b ttrue) :: gamma ⊨ t1 : T1 ]] ->
-    [[ tvars; (x, T_equiv b tfalse) :: gamma ⊨ t2 : T2 ]] ->
+    [[ tvars; (x1, T_equiv b ttrue) :: gamma ⊨ t1 : T1 ]] ->
+    [[ tvars; (x2, T_equiv b tfalse) :: gamma ⊨ t2 : T2 ]] ->
     [[ tvars; gamma ⊨ ite b t1 t2 : T_ite b T1 T2 ]].
 Proof.
   unfold annotated_reducible;
     repeat step.
 
-  apply open_reducible_T_ite with x;
+  apply open_reducible_T_ite with (x1:=x1) (x2:=x2);
     repeat step;
     side_conditions.
 Qed.
